Commutative monoid canonicalisation up to an arbitrary equivalence relation

ulib/FStar.Tactics.CanonCommMonoidSimple.Equiv.fst
@@ -30,7 +30,7 @@ open FStar.Tactics.CanonCommSwaps
 *)
 
 (* Only dump when debugging is on *)
-let dump m = if debugging () then dump m
+//let dump m = if debugging () then dump m
 
 (***** Expression syntax *)
 
@@ -63,17 +63,17 @@ let select (#a:Type) (x:atom) (am:amap a) : Tot a =
 let update (#a:Type) (x:atom) (xa:a) (am:amap a) : amap a =
   (x, xa)::fst am, snd am
 
-let rec mdenote (#a:Type) (#eq:equiv a) (m:cm a eq) (am:amap a) (e:exp) : a =
+let rec mdenote (#a:Type) (eq:equiv a) (m:cm a eq) (am:amap a) (e:exp) : a =
   match e with
   | Unit -> CM?.unit m
   | Atom x -> select x am
-  | Mult e1 e2 -> CM?.mult m (mdenote m am e1) (mdenote m am e2)
+  | Mult e1 e2 -> CM?.mult m (mdenote eq m am e1) (mdenote eq m am e2)
 
-let rec xsdenote (#a:Type) (#eq:equiv a) (m:cm a eq) (am:amap a) (xs:list atom) : a =
+let rec xsdenote (#a:Type) (eq:equiv a) (m:cm a eq) (am:amap a) (xs:list atom) : a =
   match xs with
   | [] -> CM?.unit m
   | [x] -> select x am
-  | x::xs' -> CM?.mult m (select x am) (xsdenote m am xs')
+  | x::xs' -> CM?.mult m (select x am) (xsdenote eq m am xs')
 
 (***** Flattening expressions to lists of atoms *)
 
@@ -83,46 +83,46 @@ let rec flatten (e:exp) : list atom =
   | Atom x -> [x]
   | Mult e1 e2 -> flatten e1 @ flatten e2
 
-let rec flatten_correct_aux (#a:Type) (#eq:equiv a) (m:cm a eq) (am:amap a) (xs1 xs2:list atom) 
-  : Lemma (xsdenote m am (xs1 @ xs2) `EQ?.eq eq` CM?.mult m (xsdenote m am xs1)
-                                                            (xsdenote m am xs2)) = 
+let rec flatten_correct_aux (#a:Type) (eq:equiv a) (m:cm a eq) (am:amap a) (xs1 xs2:list atom) 
+  : Lemma (xsdenote eq m am (xs1 @ xs2) `EQ?.eq eq` CM?.mult m (xsdenote eq m am xs1)
+                                                               (xsdenote eq m am xs2)) = 
   match xs1 with
   | [] -> 
-      CM?.identity m (xsdenote m am xs2);
-      EQ?.symmetry eq (CM?.mult m (CM?.unit m) (xsdenote m am xs2)) (xsdenote m am xs2)
+      CM?.identity m (xsdenote eq m am xs2);
+      EQ?.symmetry eq (CM?.mult m (CM?.unit m) (xsdenote eq m am xs2)) (xsdenote eq m am xs2)
   | [x] -> (
       if (Nil? xs2) 
       then (right_identity eq m (select x am);
             EQ?.symmetry eq (CM?.mult m (select x am) (CM?.unit m)) (select x am))
-      else EQ?.reflexivity eq (CM?.mult m (xsdenote m am [x]) (xsdenote m am xs2)))
+      else EQ?.reflexivity eq (CM?.mult m (xsdenote eq m am [x]) (xsdenote eq m am xs2)))
   | x::xs1' -> 
-      flatten_correct_aux m am xs1' xs2;
+      flatten_correct_aux eq m am xs1' xs2;
       EQ?.reflexivity eq (select x am);
-      CM?.congruence m (select x am) (xsdenote m am (xs1' @ xs2)) 
-                       (select x am) (CM?.mult m (xsdenote m am xs1') (xsdenote m am xs2));
-      CM?.associativity m (select x am) (xsdenote m am xs1') (xsdenote m am xs2);
-      EQ?.symmetry eq (CM?.mult m (CM?.mult m (select x am) (xsdenote m am xs1')) (xsdenote m am xs2)) 
-                      (CM?.mult m (select x am) (CM?.mult m (xsdenote m am xs1') (xsdenote m am xs2)));
-      EQ?.transitivity eq (CM?.mult m (select x am) (xsdenote m am (xs1' @ xs2)))
-                          (CM?.mult m (select x am) (CM?.mult m (xsdenote m am xs1') (xsdenote m am xs2)))
-                          (CM?.mult m (CM?.mult m (select x am) (xsdenote m am xs1')) (xsdenote m am xs2))
+      CM?.congruence m (select x am) (xsdenote eq m am (xs1' @ xs2)) 
+                       (select x am) (CM?.mult m (xsdenote eq m am xs1') (xsdenote eq m am xs2));
+      CM?.associativity m (select x am) (xsdenote eq m am xs1') (xsdenote eq m am xs2);
+      EQ?.symmetry eq (CM?.mult m (CM?.mult m (select x am) (xsdenote eq m am xs1')) (xsdenote eq m am xs2)) 
+                      (CM?.mult m (select x am) (CM?.mult m (xsdenote eq m am xs1') (xsdenote eq m am xs2)));
+      EQ?.transitivity eq (CM?.mult m (select x am) (xsdenote eq m am (xs1' @ xs2)))
+                          (CM?.mult m (select x am) (CM?.mult m (xsdenote eq m am xs1') (xsdenote eq m am xs2)))
+                          (CM?.mult m (CM?.mult m (select x am) (xsdenote eq m am xs1')) (xsdenote eq m am xs2))
 
-let rec flatten_correct (#a:Type) (#eq:equiv a) (m:cm a eq) (am:amap a) (e:exp) 
-  : Lemma (mdenote m am e `EQ?.eq eq` xsdenote m am (flatten e)) = 
+let rec flatten_correct (#a:Type) (eq:equiv a) (m:cm a eq) (am:amap a) (e:exp) 
+  : Lemma (mdenote eq m am e `EQ?.eq eq` xsdenote eq m am (flatten e)) = 
   match e with
   | Unit -> EQ?.reflexivity eq (CM?.unit m)
   | Atom x -> EQ?.reflexivity eq (select x am)
   | Mult e1 e2 -> 
-      flatten_correct_aux m am (flatten e1) (flatten e2);
-      EQ?.symmetry eq (xsdenote m am (flatten e1 @ flatten e2)) 
-                      (CM?.mult m (xsdenote m am (flatten e1)) (xsdenote m am (flatten e2)));
-      flatten_correct m am e1; 
-      flatten_correct m am e2;
-      CM?.congruence m (mdenote m am e1) (mdenote m am e2) 
-                       (xsdenote m am (flatten e1)) (xsdenote m am (flatten e2));
-      EQ?.transitivity eq (CM?.mult m (mdenote m am e1) (mdenote m am e2)) 
-                          (CM?.mult m (xsdenote m am (flatten e1)) (xsdenote m am (flatten e2)))
-                          (xsdenote m am (flatten e1 @ flatten e2))  
+      flatten_correct_aux eq m am (flatten e1) (flatten e2);
+      EQ?.symmetry eq (xsdenote eq m am (flatten e1 @ flatten e2)) 
+                      (CM?.mult m (xsdenote eq m am (flatten e1)) (xsdenote eq m am (flatten e2)));
+      flatten_correct eq m am e1; 
+      flatten_correct eq m am e2;
+      CM?.congruence m (mdenote eq m am e1) (mdenote eq m am e2) 
+                       (xsdenote eq m am (flatten e1)) (xsdenote eq m am (flatten e2));
+      EQ?.transitivity eq (CM?.mult m (mdenote eq m am e1) (mdenote eq m am e2)) 
+                          (CM?.mult m (xsdenote eq m am (flatten e1)) (xsdenote eq m am (flatten e2)))
+                          (xsdenote eq m am (flatten e1 @ flatten e2))  
 
 (***** Permuting the lists of atoms
        by swapping adjacent elements *)
@@ -131,8 +131,8 @@ let permute = list atom -> list atom
 
 // high-level correctness criterion for permutations
 let permute_correct (p:permute) =
-  #a:Type -> #eq:equiv a -> m:cm a eq -> am:amap a -> xs:list atom ->
-    Lemma (xsdenote m am xs `EQ?.eq eq` xsdenote m am (p xs))
+  #a:Type -> eq:equiv a -> m:cm a eq -> am:amap a -> xs:list atom ->
+    Lemma (xsdenote eq m am xs `EQ?.eq eq` xsdenote eq m am (p xs))
 
 // sufficient condition:
 // permutation has to be expressible as swaps of adjacent list elements
@@ -154,10 +154,10 @@ let rec apply_swap_aux (#a:Type) (n:nat) (xs:list a) (s:swap (length xs + n))
 
 let apply_swap (#a:Type) = apply_swap_aux #a 0
 
-let rec apply_swap_aux_correct (#a:Type) (n:nat) (#eq:equiv a) (m:cm a eq) (am:amap a)
+let rec apply_swap_aux_correct (#a:Type) (n:nat) (eq:equiv a) (m:cm a eq) (am:amap a)
                            (xs:list atom) (s:swap (length xs + n))
   : Lemma (requires True)
-      (ensures (xsdenote m am xs `EQ?.eq eq` xsdenote m am (apply_swap_aux n xs s)))
+      (ensures (xsdenote eq m am xs `EQ?.eq eq` xsdenote eq m am (apply_swap_aux n xs s)))
       (decreases xs) =
   match xs with
   | [] -> EQ?.reflexivity eq (CM?.unit m)
@@ -165,35 +165,35 @@ let rec apply_swap_aux_correct (#a:Type) (n:nat) (#eq:equiv a) (m:cm a eq) (am:a
   | [x1;x2] -> 
       if n = (s <: nat) 
       then CM?.commutativity m (select x1 am) (select x2 am)
-      else EQ?.reflexivity eq (xsdenote m am [x1;x2])
+      else EQ?.reflexivity eq (xsdenote eq m am [x1;x2])
   | x1 :: x2 :: xs' -> 
       if n = (s <: nat)
       then (
-        CM?.associativity m (select x1 am) (select x2 am) (xsdenote m am xs');
-        EQ?.symmetry eq (CM?.mult m (CM?.mult m (select x1 am) (select x2 am)) (xsdenote m am xs')) 
-                        (CM?.mult m (select x1 am) (CM?.mult m (select x2 am) (xsdenote m am xs')));
+        CM?.associativity m (select x1 am) (select x2 am) (xsdenote eq m am xs');
+        EQ?.symmetry eq (CM?.mult m (CM?.mult m (select x1 am) (select x2 am)) (xsdenote eq m am xs')) 
+                        (CM?.mult m (select x1 am) (CM?.mult m (select x2 am) (xsdenote eq m am xs')));
         CM?.commutativity m (select x1 am) (select x2 am);
-        EQ?.reflexivity eq (xsdenote m am xs');
-        CM?.congruence m (CM?.mult m (select x1 am) (select x2 am)) (xsdenote m am xs') 
-                         (CM?.mult m (select x2 am) (select x1 am)) (xsdenote m am xs');
-        CM?.associativity m (select x2 am) (select x1 am) (xsdenote m am xs');
-        EQ?.transitivity eq (CM?.mult m (select x1 am) (CM?.mult m (select x2 am) (xsdenote m am xs')))
-                            (CM?.mult m (CM?.mult m (select x1 am) (select x2 am)) (xsdenote m am xs'))
-                            (CM?.mult m (CM?.mult m (select x2 am) (select x1 am)) (xsdenote m am xs'));
-        EQ?.transitivity eq (CM?.mult m (select x1 am) (CM?.mult m (select x2 am) (xsdenote m am xs')))
-                            (CM?.mult m (CM?.mult m (select x2 am) (select x1 am)) (xsdenote m am xs'))
-                            (CM?.mult m (select x2 am) (CM?.mult m (select x1 am) (xsdenote m am xs'))))
+        EQ?.reflexivity eq (xsdenote eq m am xs');
+        CM?.congruence m (CM?.mult m (select x1 am) (select x2 am)) (xsdenote eq m am xs') 
+                         (CM?.mult m (select x2 am) (select x1 am)) (xsdenote eq m am xs');
+        CM?.associativity m (select x2 am) (select x1 am) (xsdenote eq m am xs');
+        EQ?.transitivity eq (CM?.mult m (select x1 am) (CM?.mult m (select x2 am) (xsdenote eq m am xs')))
+                            (CM?.mult m (CM?.mult m (select x1 am) (select x2 am)) (xsdenote eq m am xs'))
+                            (CM?.mult m (CM?.mult m (select x2 am) (select x1 am)) (xsdenote eq m am xs'));
+        EQ?.transitivity eq (CM?.mult m (select x1 am) (CM?.mult m (select x2 am) (xsdenote eq m am xs')))
+                            (CM?.mult m (CM?.mult m (select x2 am) (select x1 am)) (xsdenote eq m am xs'))
+                            (CM?.mult m (select x2 am) (CM?.mult m (select x1 am) (xsdenote eq m am xs'))))
       else (
-        apply_swap_aux_correct (n+1) m am (x2 :: xs') s;
+        apply_swap_aux_correct (n+1) eq m am (x2 :: xs') s;
         EQ?.reflexivity eq (select x1 am);
-        CM?.congruence m (select x1 am) (xsdenote m am (x2 :: xs'))
-                         (select x1 am) (xsdenote m am (apply_swap_aux (n+1) (x2 :: xs') s)))
+        CM?.congruence m (select x1 am) (xsdenote eq m am (x2 :: xs'))
+                         (select x1 am) (xsdenote eq m am (apply_swap_aux (n+1) (x2 :: xs') s)))
 
-let apply_swap_correct (#a:Type) (#eq:equiv a) (m:cm a eq) (am:amap a)
+let apply_swap_correct (#a:Type) (eq:equiv a) (m:cm a eq) (am:amap a)
                        (xs:list atom) (s:swap (length xs))
-  : Lemma (ensures (xsdenote m am xs `EQ?.eq eq` xsdenote m am (apply_swap xs s)))
+  : Lemma (ensures (xsdenote eq m am xs `EQ?.eq eq` xsdenote eq m am (apply_swap xs s)))
           (decreases xs) = 
-  apply_swap_aux_correct 0 m am xs s
+  apply_swap_aux_correct 0 eq m am xs s
 
 let rec apply_swaps (#a:Type) (xs:list a) (ss:list (swap (length xs))) 
   : Pure (list a) (requires True)
@@ -202,32 +202,32 @@ let rec apply_swaps (#a:Type) (xs:list a) (ss:list (swap (length xs)))
   | [] -> xs
   | s::ss' -> apply_swaps (apply_swap xs s) ss'
 
-let rec apply_swaps_correct (#a:Type) (#eq:equiv a) (m:cm a eq) (am:amap a)
+let rec apply_swaps_correct (#a:Type) (eq:equiv a) (m:cm a eq) (am:amap a)
                             (xs:list atom) (ss:list (swap (length xs)))
   : Lemma (requires True)
-      (ensures (xsdenote m am xs `EQ?.eq eq` xsdenote m am (apply_swaps xs ss)))
+      (ensures (xsdenote eq m am xs `EQ?.eq eq` xsdenote eq m am (apply_swaps xs ss)))
       (decreases ss) =
   match ss with
-  | [] -> EQ?.reflexivity eq (xsdenote m am xs)
+  | [] -> EQ?.reflexivity eq (xsdenote eq m am xs)
   | s::ss' -> 
-      apply_swap_correct m am xs s;
-      apply_swaps_correct m am (apply_swap xs s) ss';
-      EQ?.transitivity eq (xsdenote m am xs)
-                          (xsdenote m am (apply_swap xs s))
-                          (xsdenote m am (apply_swaps (apply_swap xs s) ss'))
+      apply_swap_correct eq m am xs s;
+      apply_swaps_correct eq m am (apply_swap xs s) ss';
+      EQ?.transitivity eq (xsdenote eq m am xs)
+                          (xsdenote eq m am (apply_swap xs s))
+                          (xsdenote eq m am (apply_swaps (apply_swap xs s) ss'))
 
 let permute_via_swaps (p:permute) =
   (#a:Type) -> (am:amap a) -> xs:list atom ->
     Lemma (exists (ss:swaps_for xs). p xs == apply_swaps xs ss)
 
 let rec permute_via_swaps_correct_aux (p:permute) (pvs:permute_via_swaps p)
-                               (#a:Type) (#eq:equiv a)(m:cm a eq) (am:amap a) (xs:list atom) 
-  : Lemma (xsdenote m am xs `EQ?.eq eq` xsdenote m am (p xs)) =
+                               (#a:Type) (eq:equiv a)(m:cm a eq) (am:amap a) (xs:list atom) 
+  : Lemma (xsdenote eq m am xs `EQ?.eq eq` xsdenote eq m am (p xs)) =
   pvs am xs;
   assert(exists (ss:swaps_for xs). p xs == apply_swaps xs ss);
-  exists_elim (xsdenote m am xs `EQ?.eq eq` xsdenote m am (p xs))
+  exists_elim (xsdenote eq m am xs `EQ?.eq eq` xsdenote eq m am (p xs))
     (() <: squash (exists (ss:swaps_for xs). p xs == apply_swaps xs ss))
-    (fun ss -> apply_swaps_correct m am xs ss)
+    (fun ss -> apply_swaps_correct eq m am xs ss)
 
 let permute_via_swaps_correct
   (p:permute) (pvs:permute_via_swaps p) : permute_correct p =
@@ -250,9 +250,9 @@ let sort_via_swaps (#a:Type) (am:amap a)  (xs:list atom)
   // but ss gets substituted by its definition in the WP
   // (the same already in FStar.Tactics.CanonCommMonoidSimple.fst)
 
-let rec sort_correct_aux (#a:Type) (#eq:equiv a) (m:cm a eq) (am:amap a) (xs:list atom) 
-  : Lemma (xsdenote m am xs `EQ?.eq eq` xsdenote m am (sort xs)) =
-  permute_via_swaps_correct sort (fun #a am -> sort_via_swaps am) m am xs
+let rec sort_correct_aux (#a:Type) (eq:equiv a) (m:cm a eq) (am:amap a) (xs:list atom) 
+  : Lemma (xsdenote eq m am xs `EQ?.eq eq` xsdenote eq m am (sort xs)) =
+  permute_via_swaps_correct sort (fun #a am -> sort_via_swaps am) eq m am xs
 
 let sort_correct : permute_correct sort = (fun #a -> sort_correct_aux #a)
 
@@ -261,31 +261,37 @@ let sort_correct : permute_correct sort = (fun #a -> sort_correct_aux #a)
 [@plugin]
 let canon (e:exp) = sort (flatten e)
 
-let canon_correct (#a:Type) (#eq:equiv a) (m:cm a eq) (am:amap a) (e:exp) 
-  : Lemma (mdenote m am e `EQ?.eq eq` xsdenote m am (canon e)) =
-  flatten_correct m am e; 
-  sort_correct m am (flatten e);
-  EQ?.transitivity eq (mdenote m am e)
-                      (xsdenote m am (flatten e))
-                      (xsdenote m am (sort (flatten e)))
+let canon_correct (#a:Type) (eq:equiv a) (m:cm a eq) (am:amap a) (e:exp) 
+  : Lemma (mdenote eq m am e `EQ?.eq eq` xsdenote eq m am (canon e)) =
+  flatten_correct eq m am e; 
+  sort_correct eq m am (flatten e);
+  EQ?.transitivity eq (mdenote eq m am e)
+                      (xsdenote eq m am (flatten e))
+                      (xsdenote eq m am (sort (flatten e)))
 
-let monoid_reflect_orig (#a:Type) (#eq:equiv a) (m:cm a eq) (am:amap a) (e1 e2:exp)
-  : Lemma (requires (xsdenote m am (canon e1) `EQ?.eq eq` xsdenote m am (canon e2)))
-          (ensures (mdenote m am e1 `EQ?.eq eq` mdenote m am e2)) =
-  canon_correct m am e1; 
-  canon_correct m am e2;
-  EQ?.symmetry eq (mdenote m am e2) (xsdenote m am (canon e2));
-  EQ?.transitivity eq (mdenote m am e1)
-                      (xsdenote m am (canon e1))
-                      (xsdenote m am (canon e2));
-  EQ?.transitivity eq (mdenote m am e1)
-                      (xsdenote m am (canon e2))
-                      (mdenote m am e2)
+let monoid_reflect_orig (#a:Type) (eq:equiv a) (m:cm a eq) (am:amap a) (e1 e2:exp)
+  : Lemma (requires (xsdenote eq m am (canon e1) `EQ?.eq eq` xsdenote eq m am (canon e2)))
+          (ensures (mdenote eq m am e1 `EQ?.eq eq` mdenote eq m am e2)) =
+  canon_correct eq m am e1; 
+  canon_correct eq m am e2;
+  EQ?.symmetry eq (mdenote eq m am e2) (xsdenote eq m am (canon e2));
+  EQ?.transitivity eq (mdenote eq m am e1)
+                      (xsdenote eq m am (canon e1))
+                      (xsdenote eq m am (canon e2));
+  EQ?.transitivity eq (mdenote eq m am e1)
+                      (xsdenote eq m am (canon e2))
+                      (mdenote eq m am e2)
 
-let monoid_reflect (#a:Type) (#eq:equiv a) (m:cm a eq) (am:amap a) (e1 e2:exp)
-    (_ : squash (xsdenote m am (canon e1) `EQ?.eq eq` xsdenote m am (canon e2)))
-       : squash (mdenote m am e1 `EQ?.eq eq` mdenote m am e2) =
-  monoid_reflect_orig #a m am e1 e2
+let monoid_reflect (#a:Type) (eq:equiv a) (m:cm a eq) (am:amap a) (e1 e2:exp)
+    (_ : squash (xsdenote eq m am (canon e1) `EQ?.eq eq` xsdenote eq m am (canon e2)))
+       : squash (mdenote eq m am e1 `EQ?.eq eq` mdenote eq m am e2) =
+  monoid_reflect_orig #a eq m am e1 e2
+
+let monoid_reflexivity (#a:Type) (eq:equiv a) (m:cm a eq) (am:amap a) (e:exp)
+  : squash ((let FStar.Algebra.CommMonoid.Equiv.EQ eq _ _ _ = 
+               eq in
+              eq) (mdenote eq m am e) (mdenote eq m am e)) =
+  EQ?.reflexivity eq (mdenote eq m am e)
 
 (* Finds the position of first occurrence of x in xs.
    This is now specialized to terms and their funny term_eq. *)
@@ -318,9 +324,50 @@ let rec reification_aux (#a:Type) (ts:list term) (am:amap a)
     then (Unit, ts, am)
     else fatom t ts am
 
-let reification (#a:Type) (#eq:equiv a) (m:cm a eq) (ts:list term) (am:amap a) (t:term) :
+let reification (#a:Type) (eq:equiv a) (m:cm a eq) (ts:list term) (am:amap a) (t:term) :
     Tac (exp * list term * amap a) =
   let mult = norm_term [delta] (quote (CM?.mult m)) in
   let unit = norm_term [delta] (quote (CM?.unit m)) in
   let t    = norm_term [delta] t in
   reification_aux ts am mult unit t
+
+let canon_monoid (#a:Type) (eq:equiv a) (m:cm a eq) : Tac unit =
+  norm [];
+  match term_as_formula (cur_goal ()) with
+  | Comp (Eq (Some t)) t1 t2 ->
+      // dump ("t1 =" ^ term_to_string t1 ^
+      //     "; t2 =" ^ term_to_string t2);
+      if term_eq t (quote a) then
+        let (r1, ts, am) = reification eq m [] (const (CM?.unit m)) t1 in
+        let (r2, _, am) = reification eq m ts am t2 in
+        // dump ("am =" ^ term_to_string (quote am));
+        change_sq (quote (mdenote eq m am r1 `EQ?.eq eq` mdenote eq m am r2));
+        // dump ("before =" ^ term_to_string (norm_term [delta;primops]
+        //   (quote (mdenote eq m am r1 `EQ?.eq eq` mdenote eq m am r2)))); 
+        // dump ("expected after =" ^ term_to_string (norm_term [delta;primops]
+        //   (quote (xsdenote eq m am (canon r1) `EQ?.eq eq`
+        //           xsdenote eq m am (canon r2)))));
+        apply (`monoid_reflect);
+        // dump ("after apply");
+        norm [delta_only [`%canon; `%xsdenote; `%flatten; `%sort;
+                `%select; `%assoc; `%fst; `%__proj__Mktuple2__item___1;
+                `%(@); `%append; `%List.Tot.Base.sortWith;
+                `%List.Tot.Base.partition; `%bool_of_compare; `%compare_of_bool;
+                `%EQ?.eq;
+           ]; primops]
+        // ;apply (`monoid_reflexivity)
+        // ;dump "done"
+      else fail "Goal should be an equality at the right monoid type"
+  | _ -> fail "Goal should be an equality"
+
+(***** Example *)
+
+let lem0 (a b c d : int) =
+  assert_by_tactic (0 + 1 + a + b + c + d + 2 == (b + 0) + 2 + d + (c + a + 0) + 1)
+  (fun _ -> canon_monoid (equality_equiv int) int_plus_cm)
+
+open FStar.Mul
+
+let _ =
+  assert_by_tactic (forall (a b c d : int). ((b + 1) * 1) * 2 * a * (c * a) * 1 == a * (b + 1) * c * a * 2)
+  (fun _ -> ignore (forall_intros()); canon_monoid (equality_equiv int) int_multiply_cm)
